Remove old prove_from_known_elabs, update all proofs

src/Pyrosome/Lang/CombinedThm.v
@@ -1,5 +1,3 @@
-Set Implicit Arguments.
-
 Require Import Datatypes.String Lists.List.
 Import ListNotations.
 Open Scope string.
@@ -8,10 +6,14 @@ From Utils Require Import Utils GallinaHintDb.
 From Pyrosome Require Import Theory.Core Compilers.SemanticsPreservingDef
   Compilers.Compilers Compilers.CompilerFacts
   Elab.Elab Elab.ElabCompilers
-  Tools.AllConstructors Tools.Matches Tools.CompilerTools Compilers.CompilerTransitivity
+  Tools.CompilerTools Compilers.CompilerTransitivity
+  Tools.Matches Tools.EGraph.Automation
+  Tools.EGraph.TypeInference
+  Tools.EGraph.ComputeWf
   Tools.Resolution.
-From Pyrosome.Lang Require Import SimpleVSubst SimpleVCPS SimpleEvalCtx SimpleEvalCtxCPS
-  SimpleUnit NatHeap SimpleVCPS SimpleVCPSHeap
+From Pyrosome.Lang Require Import
+  PolySubst SimpleVSubst SimpleVCPS SimpleEvalCtx SimpleEvalCtxCPS
+  SimpleUnit NatHeap SimpleVCPS SimpleVCPSHeap Let
   SimpleVFixCPS SimpleVFixCC SimpleVCC SimpleVSTLC SimpleVCCHeap SimpleVFix.
 Import Core.Notations.
 (*TODO: repackage this in compilers*)
@@ -19,10 +21,7 @@ Import CompilerDefs.Notations.
 
 Require Coq.derive.Derive.
 
-
 Local Notation compiler_case := (compiler_case string (tgt_term:=term) (tgt_sort:=sort)).
-
-(*TODO: put in right place*)
 
 (*TODO: move to compilerdefs.v*)
 #[export] Instance compiler_case_Eqb : Eqb compiler_case :=
@@ -45,20 +44,9 @@ Proof.
     basic_core_crush.
 Qed.
 
-(*TODO: put these hints with their subjects*)
-#[local] Hint Resolve cps_preserving : elab_pfs.
-#[local] Hint Resolve Ectx_cps_preserving : elab_pfs.
-#[local] Hint Resolve fix_cps_preserving : elab_pfs.
-
 #[local] Hint Resolve ElabCompilers.elab_preserving_compiler_nil : auto_elab.
 
 #[local] Hint Resolve incl_nil_l : utils.
-  
-Ltac solve_compiler_lookup :=
-  eapply preserving_compiler_embed;
-            [ solve[ eapply elab_compiler_implies_preserving; eauto with elab_pfs auto_elab]
-            | shelve].
-  
 
 Lemma wf_lang_concat {V} `{Eqb_ok V} `{WithDefault V} (l : Rule.lang V) l1 l2
   : wf_lang_ext l l1 ->
@@ -70,31 +58,12 @@ Proof.
 Qed.
 #[local] Hint Resolve wf_lang_concat : lang_core.
 
-(*TODO: duplicated; backport above lemma*)
-Ltac prove_from_known_elabs :=
-  rewrite <- ?as_nth_tail;
-   repeat
-    lazymatch goal with
-    | |- wf_lang_ext ?l_pre (?l1 ++ ?l2) => apply wf_lang_concat
-    | |- wf_lang_ext _ [] => apply wf_lang_nil
-    | |- wf_lang_ext _ _ => prove_ident_from_known_elabs
-    | |- all_fresh _ => compute_all_fresh
-    | |- incl _ _ => compute_incl
-    end.
 
 Definition src_ext := (SimpleVFix.fix_lang++SimpleVSTLC.stlc++ heap_ctx++ eval_ctx++heap_ops++(unit_lang ++ heap ++ nat_exp ++ nat_lang)).
 
 Definition ir_ext :=
   fix_cps_lang++heap_cps_ops++(unit_lang ++ heap ++ nat_exp ++ nat_lang)
                             ++cps_lang++cps_prod_lang.
-  (*heap_cps_ops
-         ++ fix_cps_lang
-         ++ cps_lang
-         ++ cps_prod_lang
-         ++ unit_lang
-         ++ heap
-         ++ nat_exp
-         ++ nat_lang.*)
 
 Definition tgt_ext :=
   fix_cc_lang ++ heap_cps_ops ++cc_lang ++ forget_eq_wkn ++ unit_eta ++ unit_lang
@@ -102,46 +71,13 @@ Definition tgt_ext :=
                    forget_eq_wkn'++
                    cps_prod_lang.
 
-Definition entry_ty (p : lang * compiler * compiler * lang) :=
-  preserving_compiler_ext (tgt_Model:=core_model (fst (fst (fst p))))
-    (snd (fst (fst p))) (snd (fst p)) (snd p).
-
-Create HintDb preserving_compiler_db discriminated.
-
-(* TODO: move these to their defining files, adoptthis pattern generally.*)
-#[local] Definition fix_cps_entry :=
-  mkEntry (exist entry_ty (_,_,_,_) (elab_compiler_implies_preserving fix_cps_preserving)).
-Hint Resolve fix_cps_entry : preserving_compiler_db.
-#[local] Definition cps_entry :=
-  mkEntry (exist entry_ty (_,_,_,_) SimpleVCPS.cps_preserving).
-Hint Resolve cps_entry : preserving_compiler_db.
-#[local] Definition heap_ctx_cps_entry :=
-  mkEntry (exist entry_ty (_,_,_,_) (elab_compiler_implies_preserving heap_ctx_cps_preserving)).
-Hint Resolve heap_ctx_cps_entry : preserving_compiler_db.
-#[local] Definition Ectx_cps_entry :=
-  mkEntry (exist entry_ty (_,_,_,_) (elab_compiler_implies_preserving Ectx_cps_preserving)).
-Hint Resolve Ectx_cps_entry : preserving_compiler_db.
-#[local] Definition heap_cps_entry :=
-  mkEntry (exist entry_ty (_,_,_,_) (elab_compiler_implies_preserving heap_cps_preserving)).
-Hint Resolve heap_cps_entry : preserving_compiler_db.
-#[local] Definition heap_id_entry :=
-  mkEntry (exist entry_ty (_,_,_,_) (elab_compiler_implies_preserving cps_preserving)).
-Hint Resolve heap_id_entry : preserving_compiler_db.
-#[local] Definition cps_subst_entry :=
-  mkEntry (exist entry_ty (_,_,_,_) cps_subst_preserving).
-Hint Resolve cps_subst_entry : preserving_compiler_db.
-
-(*TODO: add let*)
 Lemma full_cps_compiler_preserving
   : preserving_compiler_ext
       (tgt_Model := core_model (ir_ext ++ block_subst ++ value_subst))
       []
-      (fix_cps++ cps ++ heap_ctx_cps ++ Ectx_cps++ heap_cps++heap_id++cps_subst++[])
-      (src_ext++exp_subst ++ value_subst).
-Proof.
-  let db := hint_db_list preserving_compiler_db in
-  prove_by_cmp_db (db_append_cmp_list (V:=string) db).
-Qed.
+      (let_cps ++fix_cps++ cps ++ heap_ctx_cps ++ Ectx_cps++ heap_cps++heap_id++cps_subst++[])
+      (let_lang++ src_ext++exp_subst ++ value_subst).
+Proof. prove_by_cmp_db. Qed.
 
 Lemma full_cc_compiler_preserving
   : preserving_compiler_ext
@@ -149,30 +85,20 @@ Lemma full_cc_compiler_preserving
       []
       (fix_cc++heap_cc++heap_id'++cc++prod_cc_compile++subst_cc++[])
       (ir_ext++block_subst ++ value_subst).
-Proof.
-  let db := constr:(db_append_cmp_list
-        [
-          exist _ (_,_,_,_) (elab_compiler_implies_preserving fix_cc_preserving);
-          exist _ (_,_,_,_) (elab_compiler_implies_preserving heap_cc_preserving);
-          exist _ (_,_,_,_) (elab_compiler_implies_preserving heap_id'_preserving);
-          exist _ (_,_,_,_) (elab_compiler_implies_preserving cc_preserving); 
-          exist _ (_,_,_,_) (elab_compiler_implies_preserving prod_cc_preserving);
-          exist _ (_,_,_,_) (elab_compiler_implies_preserving subst_cc_preserving)
-        ]) in
-  prove_by_cmp_db db.
-Qed.
+Proof. prove_by_cmp_db. Qed.
 
 Lemma full_compiler_preserving
   : preserving_compiler_ext
       (tgt_Model := core_model (tgt_ext ++ block_subst ++ value_subst))
       []
       (compile_cmp (fix_cc++heap_cc++heap_id'++cc++prod_cc_compile++subst_cc++[])
-         (fix_cps++ cps ++ heap_ctx_cps ++ Ectx_cps++ heap_cps++heap_id++cps_subst++[]))
-      (src_ext++exp_subst ++ value_subst).
+         (let_cps++fix_cps++ cps ++ heap_ctx_cps
+            ++ Ectx_cps++ heap_cps++heap_id++cps_subst++[]))
+      (let_lang ++ src_ext++exp_subst ++ value_subst).
 Proof.
   apply preservation_transitivity
         with (ir:=ir_ext ++ block_subst ++ value_subst).
-  all: try (rewrite <-?app_assoc; solve[unfold src_ext, ir_ext, tgt_ext; prove_from_known_elabs]).
+  all: try (rewrite <-?app_assoc; solve[unfold src_ext, ir_ext, tgt_ext;prove_by_lang_db]).
   all: try typeclasses eauto; try reflexivity.
   {
     apply full_cc_compiler_preserving.
@@ -183,8 +109,6 @@ Proof.
     compute_incl.
   }
 Qed.
-
-
 
 Notation semantics_preserving tgt cmp :=
   (semantics_preserving (tgt_Model := core_model tgt)
@@ -198,20 +122,21 @@ Lemma full_compiler_semantic
   : semantics_preserving
       (tgt_ext ++ block_subst ++ value_subst)
       (compile_cmp (fix_cc++heap_cc++heap_id'++cc++prod_cc_compile++subst_cc++[])
-                   (fix_cps++ cps ++ heap_ctx_cps ++ Ectx_cps++ heap_cps++heap_id++cps_subst++[]))
-      (src_ext ++ exp_subst ++ value_subst).
+         (let_cps++fix_cps++ cps ++ heap_ctx_cps
+            ++ Ectx_cps++ heap_cps++heap_id++cps_subst++[]))
+      (let_lang++src_ext ++ exp_subst ++ value_subst).
 Proof.
   apply inductive_implies_semantic; try typeclasses eauto;
     eauto using ModelImpls.core_model_ok; try reflexivity.
   1: apply ModelImpls.core_model_ok; try typeclasses eauto.
-  1: solve [unfold src_ext, ir_ext, tgt_ext; prove_from_known_elabs].
-  1: solve [unfold src_ext, ir_ext, tgt_ext; prove_from_known_elabs].
+  1: solve [unfold src_ext, ir_ext, tgt_ext; prove_by_lang_db].
+  1: solve [unfold src_ext, ir_ext, tgt_ext; prove_by_lang_db].
   apply full_compiler_preserving.
 Qed.
 
 Definition full_compiler :=
   (compile_cmp (fix_cc++heap_cc++heap_id'++cc++prod_cc_compile++subst_cc++[])
-     (fix_cps++ cps ++ heap_ctx_cps ++ Ectx_cps++ heap_cps++heap_id++cps_subst++[])).
+     (let_cps++fix_cps++ cps ++ heap_ctx_cps ++ Ectx_cps++ heap_cps++heap_id++cps_subst++[])).
 
 Require Import Pyrosome.Compilers.PartialEval.
 
@@ -219,7 +144,7 @@ Definition compile_fn l c t e :=
   partial_eval _ l (compile_ctx full_compiler c) (compile_sort full_compiler t) 100 (compile full_compiler e).
 
 Lemma full_compiler_with_opt_pres_eq
-  (src := src_ext ++ exp_subst ++ value_subst)
+  (src := let_lang++src_ext ++ exp_subst ++ value_subst)
   (tgt := tgt_ext  ++ block_subst ++ value_subst)
   : forall c t e1 e2,
       eq_term src c t e1 e2 ->
@@ -236,13 +161,13 @@ Proof.
   {
     eapply full_compiler_semantic; eauto.
   }
-  1,3:subst tgt;unfold src_ext, ir_ext, tgt_ext; prove_from_known_elabs.
+  1,3:[>prove_by_lang_db ..].
   {
     eapply eq_term_wf_l; eauto; try typeclasses eauto.
-    unfold src_ext, ir_ext, tgt_ext; prove_from_known_elabs.
+    prove_by_lang_db.
   }
   {
     eapply eq_term_wf_r; eauto; try typeclasses eauto.
-    unfold src_ext, ir_ext, tgt_ext; prove_from_known_elabs.
+    prove_by_lang_db.
   }
 Qed.
