src/Pyrosome/Lang/PolyCompilers.v
@@ -1,19 +1,24 @@
-Set Implicit Arguments.
-
 Require Import Datatypes.String Lists.List.
 Import ListNotations.
 Open Scope string.
 Open Scope list.
-From Utils Require Import Utils.
-From Pyrosome Require Import Theory.Core Elab.Elab
-  Theory.Renaming
-  Tools.Matches Compilers.Parameterizer Compilers.Compilers Compilers.CompilerFacts.
+From Utils Require Import Utils GallinaHintDb.
+From Pyrosome Require Import Theory.Core 
+  Theory.Renaming Compilers.SemanticsPreservingDef
+  Compilers.Compilers Compilers.Parameterizer Compilers.CompilerFacts
+  Elab.Elab Elab.ElabCompilers
+  Tools.CompilerTools Compilers.CompilerTransitivity
+  Tools.Matches Tools.EGraph.Automation
+  Tools.EGraph.TypeInference
+  Tools.EGraph.ComputeWf
+  Tools.Resolution.
 From Pyrosome.Lang Require Import PolySubst
-  SimpleVSubst SimpleVCPS SimpleEvalCtx
+  SimpleVSubst SimpleVCPS SimpleEvalCtx Let
   SimpleEvalCtxCPS SimpleUnit NatHeap SimpleVCPSHeap
   SimpleVFixCPS SimpleVFixCC SimpleVCC SimpleVSTLC
   SimpleVCCHeap SimpleVFix CombinedThm.
 Import Core.Notations.
+Import CompilerDefs.Notations.
 
 Require Coq.derive.Derive.
 
@@ -27,15 +32,6 @@ Definition stlc_parameterized :=
                 ("exp",Some 2)]) in
   parameterize_lang "D" {{s #"ty_env"}}
     ps stlc.
-
-(*
-Definition stlc_parameterized_def :=
-  Eval compute in Rule.hide_lang_implicits
-                    (stlc_parameterized++
-                       exp_and_val_parameterized
-                       ++ty_subst_lang)
-                    stlc_parameterized.
- *)
 
 Local Definition evp' := 
     let ps := (elab_param "D" (stlc ++exp_ret ++ exp_subst_base
@@ -64,11 +60,12 @@ Proof.
     | now prove_from_known_elabs..
     | vm_compute; exact I].
 Qed.
-#[export] Hint Resolve stlc_parameterized_wf : elab_pfs.
-
+#[local] Definition stlc_parameterized_entry :=
+  lang_entry stlc_parameterized_wf.
+#[export] Hint Resolve stlc_parameterized_entry : wf_lang_db.
 
 Definition src_parameterized :=
-    let ps := (elab_param "D" (src_ext ++ exp_ret ++ exp_subst_base
+    let ps := (elab_param "D" (let_lang ++ src_ext ++ exp_ret ++ exp_subst_base
                                  ++ value_subst)
                [("sub", Some 2);
                 ("ty", Some 0);
@@ -76,11 +73,10 @@ Definition src_parameterized :=
                 ("val",Some 2);
                 ("exp",Some 2)]) in
   parameterize_lang "D" {{s #"ty_env"}}
-    ps src_ext.
-
+    ps (let_lang ++ src_ext).
 
 Local Definition evp'' := 
-    let ps := (elab_param "D" (src_ext ++exp_ret ++ exp_subst_base
+    let ps := (elab_param "D" (let_lang ++ src_ext ++exp_ret ++ exp_subst_base
                                  ++ value_subst)
                [("sub", Some 2);
                 ("ty", Some 0);
@@ -100,18 +96,6 @@ Proof.
   rewrite <- app_assoc; eauto.
 Qed.
 
-Ltac prove_from_known_elabs ::=
-  rewrite <- ?as_nth_tail;
-   repeat
-    lazymatch goal with
-    | |- wf_lang_ext ?l_pre (?l1 ++ ?l2) => apply wf_lang_concat'
-    | |- wf_lang_ext _ [] => apply wf_lang_nil
-    | |- wf_lang_ext _ _ => prove_ident_from_known_elabs
-    | |- all_fresh _ => compute_all_fresh
-    | |- incl _ _ => compute_incl
-    end.
-
-
 Lemma src_parameterized_wf
   : wf_lang_ext ((exp_parameterized++val_parameterized)
                        ++ty_env_lang)
@@ -121,15 +105,12 @@ Proof.
   eapply parameterize_lang_preserving_ext;
     try typeclasses eauto;
     [repeat t';  constructor (*TODO: include in t'*)
-    | try now prove_from_known_elabs..
+    | try now prove_by_lang_db..
     | vm_compute; exact I].
-  {
-    unfold src_ext.
-    prove_from_known_elabs.
-  }
 Qed.
-#[export] Hint Resolve src_parameterized_wf : elab_pfs.
-
+#[local] Definition src_parameterized_entry :=
+  lang_entry src_parameterized_wf.
+#[export] Hint Resolve src_parameterized_entry : wf_lang_db.
 
 (*TODO: move to a better place*)
 Definition hide_ccase_implicits {V} `{Eqb V} `{WithDefault V}
@@ -146,23 +127,7 @@ Definition hide_compiler {V} `{Eqb V} `{WithDefault V} (l : Rule.lang V)
   NamedList.named_map (hide_ccase_implicits l).
 
 
-Definition cps_full := (fix_cps++ cps ++ heap_ctx_cps ++ Ectx_cps++ heap_cps++heap_id++cps_subst++[]).
-
-(*
-Definition rule_to_param_spec (x : string) r :=
-  match r with
-  | sort_rule c args 
-  | term_rule c args _ =>
-      (idx_of x (map fst c, inb x args)
-  | sort_eq_rule c _ _
-  | term_eq_rule c _ _ _ => (idx_of c, false)
-  end. *)
-
-(*
-src = src_parameterized
-         ++exp_and_val_parameterized*)
-
-
+Definition cps_full := (let_cps++fix_cps++ cps ++ heap_ctx_cps ++ Ectx_cps++ heap_cps++heap_id++cps_subst++[]).
 
 Definition ir_parameterized :=
   let ps := (elab_param "D" (ir_ext ++ block_subst
@@ -197,21 +162,18 @@ Proof.
   eapply parameterize_lang_preserving_ext;
     try typeclasses eauto;
     [repeat t';  constructor (*TODO: include in t'*)
-    | try now prove_from_known_elabs..
+    | try now  prove_by_lang_db..
     | vm_compute; exact I].
-  {
-    unfold ir_ext.
-    prove_from_known_elabs.
-  }
 Qed.
-#[export] Hint Resolve ir_parameterized_wf : elab_pfs.
-
+#[local] Definition ir_parameterized_entry :=
+  lang_entry ir_parameterized_wf.
+#[export] Hint Resolve ir_parameterized_entry : wf_lang_db.
 
 Definition cps_parameterized :=
     (*TODO: elab_param seems to do the right thing, why is
       parameterize_compiler doing the wrong thing with it?
      *)
-    let ps := (elab_param "D" (src_ext ++ exp_ret ++ exp_subst_base
+    let ps := (elab_param "D" (let_lang ++ src_ext ++ exp_ret ++ exp_subst_base
                                  ++ value_subst)
                [("sub", Some 2);
                 ("ty", Some 0);
@@ -228,31 +190,6 @@ Definition cps_parameterized :=
     parameterize_compiler "D"
       (*firstn 44 skips the rule for ty. TODO: still necessary?*)
       pir ps cps_full.
-(*
-Definition id_ccase '(n,r) : list (string * compiler_case string) :=
-  match r with
-  | sort_rule c _ => [(n,sort_case (map fst c) (scon n (map var (map fst c))))]
-  | term_rule c _ _ => [(n,term_case (map fst c) (con n (map var (map fst c))))]
-  |_ => []
-  end.
-  
-Definition id_compiler : lang -> compiler :=
-  flat_map id_ccase.*)
-
-(*
-Lemma id_compiler_preserving (l l' : lang)
-  : incl l l' -> preserving_compiler_ext (tgt_Model:=core_model l') [] (id_compiler l) l.
-Proof.
-  induction l;
-    basic_goal_prep;
-    basic_core_crush.
-  destruct r;
-    constructor;
-    basic_goal_prep;
-    basic_core_crush.
-  1: exact IHl.
-  1:auto.
- *)
 
 Definition ty_env_cmp := id_compiler ty_env_lang.
 
@@ -266,10 +203,11 @@ Lemma ty_subst_id_compiler_correct
        ty_env_lang).
 Proof.
   apply id_compiler_preserving; try typeclasses eauto.
-  prove_from_known_elabs.
+  prove_by_lang_db.
 Qed.
-#[export] Hint Resolve ty_subst_id_compiler_correct : elab_pfs.
-     
+#[local] Definition ty_subst_id_entry :=
+  cmp_entry ty_subst_id_compiler_correct.
+#[export] Hint Resolve ty_subst_id_entry : preserving_db.     
 
 Lemma cps_parameterized_correct
   : preserving_compiler_ext
@@ -298,14 +236,15 @@ Proof.
   all: try typeclasses eauto.
   1,2:repeat t'; try constructor.
   1: eapply use_compute_all_fresh; vm_compute; exact I.
-  2:eapply full_cps_compiler_preserving.
-  1:unfold ir_ext; prove_from_known_elabs.
-  1:unfold src_ext;prove_from_known_elabs.
+  2:rewrite <- app_assoc; eapply full_cps_compiler_preserving.
+  1:prove_by_lang_db.
+  1:prove_by_lang_db.
   2: reflexivity.
-  1: vm_compute; exact I.
+  1: vm_cast_no_check I.
 Qed.
-#[export] Hint Resolve cps_parameterized_correct : elab_pfs.
-
+#[local] Definition cps_parameterized_entry :=
+  cmp_entry cps_parameterized_correct.
+#[export] Hint Resolve cps_parameterized_entry : preserving_db.
 
 Local Open Scope lang_scope.
 Definition exists_def : lang _ :=
@@ -365,13 +304,11 @@ Definition exists_def : lang _ :=
   ]
   ]}.
 
-
 #[local] Definition Exists_inst_for_db := inst_for_db "Exists".
 #[export] Hint Resolve Exists_inst_for_db : injective_con.
 
-
 Derive exists_lang
-  SuchThat (elab_lang_ext (exp_param_substs
+  in (elab_lang_ext (exp_param_substs
                              ++ exp_ty_subst
                              ++ val_param_substs
                              ++ val_ty_subst
@@ -380,10 +317,11 @@ Derive exists_lang
                              ++exp_parameterized++val_parameterized
                              ++ty_env_lang)
               exists_def exists_lang)
-       As exists_lang_wf.
+       as exists_lang_wf.
 Proof. auto_elab. Qed.
-#[export] Hint Resolve exists_lang_wf : elab_pfs. 
-
+#[local] Definition exists_lang_entry :=
+  lang_entry (elab_lang_implies_wf exists_lang_wf).
+#[export] Hint Resolve exists_lang_entry : wf_lang_db.
 
 Definition exists_block_def : lang _ :=
   {[l (*l/subst TODO: psubst*)
@@ -465,7 +403,6 @@ Definition exists_block_def : lang _ :=
   ]
   ]}.
 
-
 Derive exists_block_lang
   SuchThat (elab_lang_ext (block_param_substs
                              ++val_param_substs
@@ -477,18 +414,15 @@ Derive exists_block_lang
               exists_block_def exists_block_lang)
        As exists_block_lang_wf.
 Proof. auto_elab. Qed.
-#[export] Hint Resolve exists_block_lang_wf : elab_pfs. 
-
-Import CompilerDefs.Notations.
-
-
+#[local] Definition exists_block_lang_entry :=
+  lang_entry (elab_lang_implies_wf exists_block_lang_wf).
+#[export] Hint Resolve exists_block_lang_entry : wf_lang_db.
 
 Definition exp_ty_subst_cps_def : compiler string :=
   match # from (exp_param_substs ++ exp_ty_subst) with
   | {{e #"exp_ty_subst" "D" "D'" "g" "G" "A" "e"}} =>
       {{e #"blk_ty_subst" "g" "e"}}
   end.
-
 
 Require Import Tools.UnElab.
 
@@ -519,7 +453,9 @@ Derive ir_param_substs
               ir_param_substs)
   As ir_param_substs_wf.
 Proof. auto_elab. Qed.
-#[export] Hint Resolve ir_param_substs_wf : elab_pfs.
+#[local] Definition ir_param_substs_entry :=
+  lang_entry (elab_lang_implies_wf ir_param_substs_wf).
+#[export] Hint Resolve ir_param_substs_entry : wf_lang_db.
 
 #[local] Definition cmp' := Eval compute in cps_parameterized.
 Derive exp_ty_subst_cps
@@ -543,7 +479,9 @@ Derive exp_ty_subst_cps
               (exp_param_substs ++ exp_ty_subst))
   As exp_ty_subst_cps_preserving.
 Proof. auto_elab_compiler. Qed.
-#[export] Hint Resolve exp_ty_subst_cps_preserving : elab_pfs.
+#[local] Definition exp_ty_subst_cps_entry :=
+  cmp_entry (elab_compiler_implies_preserving exp_ty_subst_cps_preserving).
+#[export] Hint Resolve exp_ty_subst_cps_entry : preserving_db.
 
 Definition poly_cps_def : compiler string :=
   match # from poly with
@@ -651,7 +589,7 @@ Ltac intermediate_term e :=
   end.
 
 Derive poly_cps
-  SuchThat (elab_preserving_compiler
+  in (elab_preserving_compiler
               (exp_ty_subst_cps
                  ++ id_compiler (val_param_substs
                                    ++ val_ty_subst
@@ -671,22 +609,20 @@ Derive poly_cps
               poly_cps_def
               poly_cps
               poly)
-  As poly_cps_preserving.
+  as poly_cps_preserving.
 Proof.
-  change cps_parameterized with cmp'.
   auto_elab_compiler.
-  (* Automation.auto_elab_compiler. 1:36-1:44+ Why is this longer?*)
-  (*260s for legacy auto*)
-  { Automation.by_reduction; Matches.t'. }
-  Unshelve.
-  all: repeat Matches.t'.
+  { Automation.by_reduction; t'. }
+  (*Automation.auto_elab_compiler.
+12:57-1:46+; too long
+   *)  
 Qed.
-#[export] Hint Resolve poly_cps_preserving : elab_pfs.
-
+#[local] Definition poly_cps_entry :=
+  cmp_entry (elab_compiler_implies_preserving poly_cps_preserving).
+#[export] Hint Resolve poly_cps_entry : preserving_db.
 
 Local Definition unpack_swap :=
   {{e #"snoc" (#"snoc" (#"cmp" (#"cmp" #"wkn" #"wkn") #"wkn") #"hd") {ovar 2} }}.
-
 
 Definition exists_cps_def : compiler string :=
   match # from exists_lang with
@@ -725,15 +661,15 @@ Derive exists_cps
               exists_lang)
   As exists_cps_preserving.
 Proof.
-  change cps_parameterized with cmp'.
   (*TODO: takes much longer than legacy auto_elab_compiler (has not terminated). Why?
     Time  1:Automation.auto_elab_compiler.
     Legacy: ~50s
    *)
   auto_elab_compiler.
 Qed.
-#[export] Hint Resolve exists_cps_preserving : elab_pfs.
-
+#[local] Definition exists_cps_entry :=
+  cmp_entry (elab_compiler_implies_preserving exists_cps_preserving).
+#[export] Hint Resolve exists_cps_entry : preserving_db.
 
 Definition tgt_parameterized :=
   let ps := (elab_param "D" (tgt_ext ++ block_subst
@@ -768,14 +704,12 @@ Proof.
   eapply parameterize_lang_preserving_ext;
     try typeclasses eauto;
     [repeat t';  constructor (*TODO: include in t'*)
-    | try now prove_from_known_elabs..
-    | vm_compute; exact I].
-  {
-    unfold tgt_ext.
-    prove_from_known_elabs.
-  }
+    | try now prove_by_lang_db..
+    | Ltac.flagged_exact I].
 Qed.
-#[export] Hint Resolve tgt_parameterized_wf : elab_pfs.
+#[local] Definition tgt_parameterized_entry :=
+  lang_entry tgt_parameterized_wf.
+#[export] Hint Resolve tgt_parameterized_entry : wf_lang_db.
 
 Definition cc_full :=
   (fix_cc ++ heap_cc ++ heap_id' ++ cc ++ prod_cc_compile ++ subst_cc ++ []).
@@ -797,7 +731,6 @@ Definition cc_parameterized :=
                 ("blk",Some 1)]) in
     parameterize_compiler "D"
       ptgt pir cc_full.
-
 
 Lemma cc_parameterized_correct
   : preserving_compiler_ext
@@ -833,13 +766,14 @@ Proof.
       by basic_utils_crush.
     eapply full_cc_compiler_preserving.
   }
-  1: unfold tgt_ext; prove_from_known_elabs.
-  1:unfold ir_ext;prove_from_known_elabs.
+  1: prove_by_lang_db.
+  1: prove_by_lang_db.
   2: reflexivity.
-  1: vm_compute; exact I.
+  1: vm_cast_no_check I.
 Qed.
-#[export] Hint Resolve cc_parameterized_correct : elab_pfs.
-
+#[local] Definition cc_parameterized_entry :=
+  cmp_entry cc_parameterized_correct.
+#[export] Hint Resolve cc_parameterized_entry : preserving_db.
 
 Definition exists_cc_def : compiler string :=
   match # from exists_block_lang with
@@ -850,7 +784,6 @@ Definition exists_cc_def : compiler string :=
   | {{e #"unpack" "D" "G" "B" "v" "e'" }} =>
       {{e #"unpack" "v" (#"blk_subst" (#"snoc" #"forget" (#"pair" {ovar 1} #"hd")) "e")  }}
   end.
-
 
 Definition tgt_param_substs_def :=
   Eval compute in
@@ -864,8 +797,6 @@ Definition tgt_param_substs_def :=
                                  ++ ty_env_lang) in
     eqn_rules type_subst_mode deps
     (hide_lang_implicits (tgt_parameterized++deps) tgt_parameterized).
-
-
 
 Derive tgt_param_substs
   SuchThat (elab_lang_ext (tgt_parameterized
@@ -881,11 +812,11 @@ Derive tgt_param_substs
               tgt_param_substs)
   As tgt_param_substs_wf.
 Proof. auto_elab. Qed.
-#[export] Hint Resolve tgt_param_substs_wf : elab_pfs.
-
+#[local] Definition tgt_param_substs_entry :=
+  lang_entry (elab_lang_implies_wf tgt_param_substs_wf).
+#[export] Hint Resolve tgt_param_substs_entry : wf_lang_db.
 
 #[local] Definition cmp'' := Eval compute in cc_parameterized.
-
 
 Definition block_ty_subst_cc_def : compiler string :=
   match # from (block_param_substs
@@ -919,8 +850,10 @@ Derive block_ty_subst_cc
               (block_param_substs ++ val_param_substs
                  ++ block_ty_subst++env_ty_subst))
   As block_ty_subst_cc_preserving.
-Proof. auto_elab_compiler. Qed.
-#[export] Hint Resolve block_ty_subst_cc_preserving : elab_pfs.
+Proof. Automation.auto_elab_compiler. Qed.
+#[local] Definition block_ty_subst_cc_entry :=
+  cmp_entry (elab_compiler_implies_preserving block_ty_subst_cc_preserving).
+#[export] Hint Resolve block_ty_subst_cc_entry : preserving_db.
 
 Derive exists_cc
   SuchThat (elab_preserving_compiler
@@ -945,7 +878,8 @@ Derive exists_cc
 Proof.
   auto_elab_compiler.
   { Automation.by_reduction; Matches.t'. }
-  {   
+  {
+    
     compute_eq_compilation.
     reduce.
     hide_implicits.
@@ -960,7 +894,7 @@ Proof.
     1: sort_cong.
     all: try term_refl.
     all:compute_eq_compilation.
-    1:by_reduction.
+    1:by_reduction; t'.
     hide_implicits.
     term_cong.
     all:compute_eq_compilation.
@@ -987,7 +921,9 @@ Proof.
   Unshelve.
   all:repeat Matches.t'.
 Qed.
-#[export] Hint Resolve exists_cc_preserving : elab_pfs.
+#[local] Definition exists_cc_cmp_entry :=
+  cmp_entry (elab_compiler_implies_preserving exists_cc_preserving).
+#[export] Hint Resolve exists_cc_cmp_entry : preserving_db.
 
 Require Import Pyrosome.Compilers.CompilerTransitivity.
 
@@ -1001,6 +937,7 @@ Require Import Pyrosome.Compilers.CompilerTransitivity.
       rewrite flat_map_app.
       auto.
     Qed.
+    
 Lemma id_compiler_preserving'  (l_pre l l' : lang)
   : wf_lang l_pre ->
     wf_lang_ext l_pre l -> incl l l' ->
@@ -1081,13 +1018,14 @@ Proof.
                       ++env_ty_subst
                       ++ty_subst_lang)).
 Lemma ty_subst_lang_id_ext
-  : elab_preserving_compiler
+  : preserving_compiler_ext
       (cps_parameterized ++ ty_env_cmp)
-      (((val_param_substs
+      (tgt_Model := core_model ((val_param_substs
                       ++ val_ty_subst
                       ++env_ty_subst
-                      ++ty_subst_lang)++ val_parameterized ++ ty_env_lang))
-      id_cps_def
+                      ++ty_subst_lang)
+                                  ++ ir_parameterized ++ block_parameterized
+                                  ++ val_parameterized ++ ty_env_lang))
       (id_compiler (val_param_substs
                       ++ val_ty_subst
                       ++env_ty_subst
@@ -1096,21 +1034,13 @@ Lemma ty_subst_lang_id_ext
             ++ val_ty_subst
             ++env_ty_subst
             ++ty_subst_lang).
-Proof. 
-  cleanup_elab_after
-    (  match goal with
-  | |- elab_preserving_compiler _ ?tgt ?cmp ?ecmp ?src =>
-        rewrite (as_nth_tail cmp); rewrite (as_nth_tail ecmp); rewrite (as_nth_tail src);
-         assert (wf_lang tgt) by prove_from_known_elabs
-       end; break_preserving).
-  
-  all:repeat
-    ([>repeat Matches.t; cleanup_elab_after try (try decompose_sort_eq; (solve [ by_reduction ]))
-     | .. ]).
-  Unshelve.
-  all:repeat Matches.t'.
+Proof.
+   compute_preserving_compiler
+         (src_parameterized ++ exp_parameterized
+            ++ val_parameterized ++ ty_env_lang).
 Qed.
-#[export] Hint Resolve ty_subst_lang_id_ext :elab_pfs.
+#[local] Definition ty_subst_lang_id_ext_entry := cmp_entry ty_subst_lang_id_ext.
+#[export] Hint Resolve ty_subst_lang_id_ext_entry : preserving_db.
 
 #[local] Definition id_cc_def :=
         Eval compute in
@@ -1118,46 +1048,47 @@ Qed.
           (ty_subst_lang++ val_parameterized ++ ty_env_lang)
           (id_compiler ty_subst_lang).
 
-  Lemma ty_subst_lang_id_ext_cc
-  : elab_preserving_compiler
+Lemma ty_subst_lang_id_ext_cc
+  : preserving_compiler_ext
       (cc_parameterized ++ty_env_cmp)
-      (ty_subst_lang ++ val_parameterized ++ ty_env_lang)
-      id_cc_def
+      (tgt_Model := core_model ((val_param_substs
+                      ++ val_ty_subst
+                      ++env_ty_subst
+                      ++ty_subst_lang)
+                                  ++ tgt_parameterized ++ block_parameterized
+                                  ++ val_parameterized ++ ty_env_lang))
       (id_compiler ty_subst_lang)
-         (ty_subst_lang).
-Proof. 
-  cleanup_elab_after
-    (  match goal with
-  | |- elab_preserving_compiler _ ?tgt ?cmp ?ecmp ?src =>
-        rewrite (as_nth_tail cmp); rewrite (as_nth_tail ecmp); rewrite (as_nth_tail src);
-         assert (wf_lang tgt) by prove_from_known_elabs
-       end; break_preserving).
-  
-  all:repeat
-    ([>repeat Matches.t; cleanup_elab_after try (try decompose_sort_eq; (solve [ by_reduction ]))
-     | .. ]).
-  Unshelve.
-  all:repeat Matches.t'.
+      (ty_subst_lang).
+Proof.
+  compute_preserving_compiler (ir_parameterized ++ block_parameterized
+                                 ++ val_parameterized ++ ty_env_lang).
 Qed.
-#[export] Hint Resolve ty_subst_lang_id_ext_cc :elab_pfs.
-
+#[local] Definition ty_subst_lang_id_ext_cc_entry :=
+  cmp_entry ty_subst_lang_id_ext_cc.
+#[export] Hint Resolve ty_subst_lang_id_ext_cc_entry : preserving_db.
 
 Lemma ir_param_substs_preserving
-  :elab_preserving_compiler
+  : preserving_compiler_ext
      (block_ty_subst_cc ++ id_compiler ty_subst_lang ++ cc_parameterized ++ ty_env_cmp)
-     (tgt_param_substs ++
+     (tgt_Model := core_model (tgt_param_substs ++
         tgt_parameterized ++
         block_param_substs ++
         val_param_substs ++
         block_ty_subst ++
         env_ty_subst ++ ty_subst_lang ++ block_parameterized
-        ++ val_parameterized ++ ty_env_lang)
-     []
+        ++ val_parameterized ++ ty_env_lang))
      []
      ir_param_substs.
 Proof.
-  auto_elab_compiler.
+  compute_preserving_compiler
+    ((block_param_substs ++ val_param_substs ++ block_ty_subst ++ env_ty_subst)
+       ++ ty_subst_lang ++
+       (ir_parameterized ++ block_parameterized ++ val_parameterized)
+       ++ ty_env_lang).
 Qed.
+#[local] Definition ir_param_substs_cmp_entry :=
+  cmp_entry ir_param_substs_preserving.
+#[export] Hint Resolve ir_param_substs_cmp_entry : preserving_db.
 
 Definition poly_tgt :=
   (exists_block_lang ++
@@ -1198,52 +1129,6 @@ Definition pcc :=
     ++ block_ty_subst_cc
     ++ id_compiler ty_subst_lang ++ cc_parameterized ++ ty_env_cmp.
 
-From Pyrosome Require Import Tools.Resolution.
-
-#[local] Definition db :=
-      Eval vm_compute in
-      db_append_lang_list
-        [ exist _ (_,_) (elab_lang_implies_wf exists_lang_wf);
-          exist _ (_,_) (elab_lang_implies_wf poly_wf);
-          exist _ (_,_) (elab_lang_implies_wf exp_param_substs_wf);
-          exist _ (_,_) (elab_lang_implies_wf exp_ty_subst_wf);
-          exist _ (_,_) (elab_lang_implies_wf val_param_substs_wf);
-          exist _ (_,_) (elab_lang_implies_wf val_ty_subst_wf);
-          exist _ (_,_) (elab_lang_implies_wf env_ty_subst_wf);
-          exist _ (_,_) (elab_lang_implies_wf ty_subst_wf);
-          exist _ (_,_) src_parameterized_wf;
-          exist _ (_,_) (elab_lang_implies_wf exp_parameterized_wf);
-          exist _ (_,_) (elab_lang_implies_wf val_parameterized_wf);
-          exist _ (_,_) (elab_lang_implies_wf ty_env_wf);
-          exist _ (_,_) (elab_lang_implies_wf exists_block_lang_wf);
-          exist _ (_,_) (elab_lang_implies_wf ir_param_substs_wf);
-          exist _ (_,_) (elab_lang_implies_wf block_param_substs_wf);
-          exist _ (_,_) (elab_lang_implies_wf val_param_substs_wf);            
-          exist _ (_,_) (elab_lang_implies_wf block_ty_subst_wf);
-          exist _ (_,_) (elab_lang_implies_wf env_ty_subst_wf);
-          exist _ (_,_) (elab_lang_implies_wf ty_subst_wf);            
-          exist _ (_,_) ir_parameterized_wf;
-          exist _ (_,_) (elab_lang_implies_wf block_parameterized_wf);
-          exist _ (_,_) (elab_lang_implies_wf tgt_param_substs_wf);
-          exist _ (_,_) tgt_parameterized_wf
-        ].
-
-#[local] Definition cmp_db :=
-      Eval vm_compute in
-      db_append_cmp_list
-        [
-          exist _ (_,_,_,_) (elab_compiler_implies_preserving exists_cc_preserving);
-          exist _ (_,_,_,_) (elab_compiler_implies_preserving block_ty_subst_cc_preserving);
-          exist _ (_,_,_,_) (elab_compiler_implies_preserving ty_subst_lang_id_ext_cc);
-          exist _ (_,_,_,_) cc_parameterized_correct;
-          exist _ (_,_,_,_) (elab_compiler_implies_preserving ir_param_substs_preserving);
-          exist _ (_,_,_,_) ty_subst_id_compiler_correct;
-          exist _ (_,_,_,_) (elab_compiler_implies_preserving exists_cps_preserving);
-          exist _ (_,_,_,_) (elab_compiler_implies_preserving poly_cps_preserving);
-          exist _ (_,_,_,_) (elab_compiler_implies_preserving exp_ty_subst_cps_preserving);
-          exist _ (_,_,_,_) (elab_compiler_implies_preserving ty_subst_lang_id_ext);
-          exist _ (_,_,_,_) cps_parameterized_correct
-        ].
 
 Theorem combined_poly
   :  preserving_compiler_ext
@@ -1255,6 +1140,6 @@ Proof.
   apply preservation_transitivity
     with (ir:=poly_ir).
   all: try typeclasses eauto; try reflexivity.
-  1-3:prove_by_lang_db db.
-  1-2:prove_by_cmp_db cmp_db.
+  1-3:[>prove_by_lang_db..].
+  1-2:[>prove_by_cmp_db..].
 Qed.
