src/Pyrosome/Lang/SimpleVFix.v
@@ -1,11 +1,13 @@
-Set Implicit Arguments.
 
 Require Import Datatypes.String Lists.List.
 Import ListNotations.
 Open Scope string.
 Open Scope list.
 From Utils Require Import Utils.
-From Pyrosome Require Import Theory.Core Elab.Elab Tools.Matches Lang.SimpleVSubst Lang.SimpleVSTLC.
+From Pyrosome Require Import Theory.Core Elab.Elab
+  Tools.Matches
+  Tools.EGraph.TypeInference Tools.Resolution Tools.EGraph.ComputeWf.
+From Pyrosome.Lang Require Import PolySubst SimpleVSubst SimpleVSTLC.
 Import Core.Notations.
 
 Require Coq.derive.Derive.
@@ -31,9 +33,17 @@ Definition fix_def : lang :=
   ]
   ]}.
 
-Derive fix_lang
-       SuchThat (elab_lang_ext (stlc++exp_subst++value_subst) fix_def fix_lang)
-       As fix_wf.
-Proof. auto_elab. Qed.
-#[export] Hint Resolve fix_wf : elab_pfs.
+Definition fix_injectivity :=
+  [("fix", ["B"; "A"; "G"])].
+
+Definition fix_lang :=
+  Eval vm_compute in
+    (infer_lang_ext_simple (stlc++exp_subst++value_subst) fix_def
+       (fix_injectivity++stlc_injectivity
+          ++exp_subst_injectivity++value_subst_injectivity)).
+
+Lemma fix_wf : wf_lang_ext (stlc++exp_subst++value_subst) fix_lang.
+Proof. compute_wf_lang. Qed.
+#[local] Definition fix_entry := lang_entry fix_wf.
+#[export] Hint Resolve fix_entry : wf_lang_db.
 
