src/Utils/Result.v
@@ -1,4 +1,8 @@
-From coqutil Require Import Datatypes.Result.
+From Stdlib Require Import String.
+From coqutil Require Import Datatypes.Result Datatypes.dlist.
+From Utils Require Import Monad.
+
+Open Scope string.
 
 (*TODO: is there a better place for this?
   Used to put some info in the type of a failing computation.
@@ -16,3 +20,46 @@ Definition Some_or {A} (b:option A) els : result A :=
   | None => els
   end.
 
+Definition resultT (M : Type -> Type) A := M (result A).
+
+#[export] Instance resultT_trans : MonadTrans resultT :=
+  {|
+    transformer_monad M _ :=
+      {|
+        Mret _ a := (Mret (Success a));
+        Mbind _ _ f :=
+          Mbind (M:=M) (fun ma => match ma with
+                                      | Success a => f a
+                                      | Failure err => Mret (Failure err)
+                                      end)
+      |};
+  lift M _ A ma := @! let a <- ma in ret Success a
+  |}.
+
+
+Definition result_monad : Monad result :=
+  Eval cbv in (resultT_trans.(transformer_monad) : Monad (resultT id)).
+#[export] Existing Instance result_monad.
+
+
+Polymorphic Fixpoint dapp (l1 l2 : dlist) :=
+  match l1 with
+  | dnil => l2
+  | dcons x l1 => dcons x (dapp l1 l2)
+  end.
+
+Section __.
+  Context {A B} (comp : A -> result B).
+
+  Polymorphic Fixpoint res_exists'  l acc : result B :=
+    match l with
+    | nil => Failure acc
+    | cons x l =>
+        match comp x with
+        | Success x => Success x
+        | Failure err => res_exists' l (dapp err (dcons "|" acc))
+        end
+    end.
+
+  Polymorphic Definition res_exists l := res_exists' l dnil.
+End __.
