src/Pyrosome/Lang/SimpleVFixCC.v
@@ -1,21 +1,20 @@
-Set Implicit Arguments.
-
 Require Import Datatypes.String Lists.List.
 Import ListNotations.
 Open Scope string.
 Open Scope list.
-From Utils Require Import Utils.
-From Pyrosome Require Import Theory.Core Elab.Elab Elab.ElabCompilers Tools.Matches.
-From Pyrosome.Lang Require Import SimpleVSubst SimpleVSTLC SimpleVCPS SimpleVFix SimpleVFixCPS SimpleVCC SimpleUnit.
+From Utils Require Import Utils GallinaHintDb.
+From Pyrosome Require Import Theory.Core Compilers.Compilers
+  Elab.Elab Elab.ElabCompilers Tools.Matches Tools.EGraph.Automation
+  Tools.EGraph.TypeInference
+  Tools.EGraph.ComputeWf
+  Tools.Resolution.
+From Pyrosome.Lang Require Import
+  PolySubst SimpleVSubst SimpleVSTLC SimpleVCPS SimpleVFix SimpleVFixCPS SimpleVCC SimpleUnit.
 Import Core.Notations.
 (*TODO: repackage this in compilers*)
 Import CompilerDefs.Notations.
 
 Require Coq.derive.Derive.
-
-
-Require Import Tools.EGraph.Automation.
-
 
 Definition fix_cc_lang_def : lang :=
   {[l/subst [(cc_lang++prod_cc ++ cps_prod_lang ++ block_subst ++value_subst)]
@@ -41,10 +40,8 @@ Derive fix_cc_lang
                                fix_cc_lang)
        As fix_cc_wf.
 Proof. auto_elab. Qed.
-#[export] Hint Resolve fix_cc_wf : elab_pfs.
-
-
-
+#[local] Definition fix_cc_entry := lang_entry (elab_lang_implies_wf fix_cc_wf).
+#[export] Hint Resolve fix_cc_entry : wf_lang_db.
 
 Definition fix_cc_def : compiler :=
   match # from (fix_cps_lang) with
@@ -74,6 +71,8 @@ Derive fix_cc
                                           fix_cps_lang)
        As fix_cc_preserving.
 Proof.
-  auto_elab_compiler' (rule_named_in cc_bidirectional_rules) empty_inj_rules fail.
+  auto_elab_compiler' (rule_named_in cc_bidirectional_rules) empty_inj_rules.
 Qed.
-#[export] Hint Resolve fix_cc_preserving : elab_pfs.
+#[local] Definition fix_cc_cmp_entry :=
+  cmp_entry (elab_compiler_implies_preserving fix_cc_preserving).
+#[export] Hint Resolve fix_cc_cmp_entry : preserving_db.
