src/Pyrosome/Lang/SimpleVFixCPS.v
@@ -1,12 +1,15 @@
-Set Implicit Arguments.
-
 Require Import Datatypes.String Lists.List.
 Import ListNotations.
 Open Scope string.
 Open Scope list.
-From Utils Require Import Utils.
-From Pyrosome Require Import Theory.Core Compilers.Compilers Elab.Elab Elab.ElabCompilers Tools.Matches.
-From Pyrosome.Lang Require Import SimpleVSubst SimpleVSTLC SimpleVCPS SimpleVFix.
+From Utils Require Import Utils GallinaHintDb.
+From Pyrosome Require Import Theory.Core Compilers.Compilers
+  Elab.Elab Elab.ElabCompilers Tools.Matches Tools.EGraph.Automation
+  Tools.EGraph.TypeInference
+  Tools.EGraph.ComputeWf
+  Tools.Resolution.
+From Pyrosome.Lang Require Import
+  PolySubst SimpleVSubst SimpleVSTLC SimpleVCPS SimpleVFix.
 Import Core.Notations.
 (*TODO: repackage this in compilers*)
 Import CompilerDefs.Notations.
@@ -14,7 +17,6 @@ Import CompilerDefs.Notations.
 Require Coq.derive.Derive.
 
 Notation compiler := (compiler string).
-
 
 Definition fix_cps_lang_def : lang :=
   {[l/subst [cps_lang ++ block_subst ++ value_subst]
@@ -34,14 +36,12 @@ Definition fix_cps_lang_def : lang :=
       : #"blk" "G"
   ] ]}.
 
-
 Derive fix_cps_lang
        SuchThat (elab_lang_ext (cps_lang ++ block_subst ++ value_subst) fix_cps_lang_def fix_cps_lang)
        As fix_wf.
 Proof. auto_elab. Qed.
-#[export] Hint Resolve fix_wf : elab_pfs.
-
-
+#[local] Definition fix_cps_entry := lang_entry (elab_lang_implies_wf fix_wf).
+#[export] Hint Resolve fix_cps_entry : wf_lang_db.
 
 Definition fix_cps_def : compiler :=
   match # from (fix_lang) with
@@ -50,7 +50,6 @@ Definition fix_cps_def : compiler :=
         (#"pm_pair" #"hd"
           (#"blk_subst" {under (under {{e #"wkn"}})} "e"))}}
   end.
-
 
 Derive fix_cps
        SuchThat (elab_preserving_compiler (cps++cps_subst)
@@ -64,4 +63,6 @@ Derive fix_cps
                                           fix_lang)
        As fix_cps_preserving.
 Proof. auto_elab_compiler. Qed.
-#[export] Hint Resolve fix_cps_preserving : elab_pfs.
+#[local] Definition fix_cps_cmp_entry :=
+  cmp_entry (elab_compiler_implies_preserving fix_cps_preserving).
+#[export] Hint Resolve fix_cps_cmp_entry : preserving_db.
